More examples of Acorn programs, some fixes in the translation related to de Bruijn indices

AcornExamples.v
@@ -1,4 +1,4 @@
-(** * Examples of contracts originating from the actual Acorn contracts *)
+(** * Examples of library code and contracts originating from the actual Acorn implementation  *)
 Require Import ZArith.
 Require Import String.
 Require Import Ast CustomTactics.
@@ -27,15 +27,17 @@ Fixpoint translateDefs Σ (es : list (string * expr)) :=
   | [] => tmPrint "Done."
   | (name, e) :: es' =>
     coq_expr <- tmEval all (expr_to_term Σ (reindexify 0 e)) ;;
-    tm <- tmUnquote coq_expr ;;
+    (* tm <- tmUnquote coq_expr ;; *)
     def_txt <- tmEval all ("Definition " ++ name ++ " :=");;
-    def_ty <- tmEval all (my_projT1 tm);;
-    def <- tmEval cbn (my_projT2 tm);;
+    (* def_ty <- tmEval all (my_projT1 tm);; *)
+    (* def <- tmEval cbn (my_projT2 tm);; *)
     (* tmDefinition name def;; *)
+    print_nf name;;
+    print_nf coq_expr;;
     tmMkDefinition name coq_expr;;
-    tmPrint def_txt;;
-    tmPrint def_ty;;
-    tmPrint def;;
+    (* tmPrint def_txt;; *)
+    (* tmPrint def_ty;; *)
+    (* tmPrint def;; *)
     translateDefs Σ es'
   end.
 
@@ -67,6 +69,81 @@ End AcornMaybe.
 Import AcornMaybe.
 
 Print isJust.
+
+Module AcornProd.
+
+  Definition AP_data := [gdInd "Pair" 2 [("Pair_coq", [(TC.nAnon, tyRel 1);(TC.nAnon, tyRel 0)])] false].
+  (*---------------------*)
+
+  Definition AP_functions :=
+    [("fst", eTyLam "A" (eTyLam "A" (eLambda "x" ((tyApp (tyApp (tyInd "Pair") (tyRel 1)) (tyRel 0))) (eCase ((tyApp (tyApp (tyInd "Pair") (tyRel 1)) (tyRel 0)), 0) (tyRel 1) (eRel 0) [(pConstr "Pair_coq" ["x0";"x1"], eRel 1)]))));("snd", eTyLam "A" (eTyLam "A" (eLambda "x" ((tyApp (tyApp (tyInd "Pair") (tyRel 1)) (tyRel 0))) (eCase ((tyApp (tyApp (tyInd "Pair") (tyRel 1)) (tyRel 0)), 0) (tyRel 0) (eRel 0) [(pConstr "Pair_coq" ["x0";"x1"], eRel 0)]))))].
+
+  Run TemplateProgram (translateData AP_data).
+
+  Run TemplateProgram (translateDefs (StdLib.Σ ++ AP_data)%list AP_functions).
+End AcornProd.
+
+Module AcornListBase.
+  Import AcornBool.
+  Import AcornMaybe.
+  Import AcornProd.
+
+  Definition ALB_data :=  [gdInd "List" 1 [("Nil_coq", []);("Cons_coq", [(TC.nAnon, tyRel 0);(TC.nAnon, (tyApp (tyInd "List") (tyRel 0)))])] false].
+
+  (*---------------------*)
+
+  Definition ALB_functions := [("singleton", eTyLam "A" (eLambda "x" (tyRel 0) (eApp (eApp (eApp (eConstr "List" "Cons_coq") (eTy (tyRel 0))) (eRel 0)) (eApp (eConstr "List" "Nil_coq") (eTy (tyRel 0))))))
+  ;
+("foldr", eTyLam "A" (eTyLam "A" (eLambda "x" (tyArr (tyRel 1) (tyArr (tyRel 0) (tyRel 0))) (eLambda "x" (tyRel 0) (eLetIn "f" (eFix "rec" "x" ((tyApp (tyInd "List") (tyRel 1))) (tyRel 0) (eCase ((tyApp (tyInd "List") (tyRel 1)), 1) (tyRel 0) (eRel 0) [(pConstr "Nil_coq" [], eRel 2);(pConstr "Cons_coq" ["x0";"x1"], eApp (eApp (eRel 5) (eRel 1)) (eApp (eRel 3) (eRel 0)))])) (tyArr ((tyApp (tyInd "List") (tyRel 1))) (tyRel 0)) (eRel 0))))))
+ ;
+  ("map", eTyLam "A" (eTyLam "A" (eLambda "x" (tyArr (tyRel 1) (tyRel 0)) (eApp (eApp (eApp (eApp (eConst "foldr") (eTy (tyRel 1))) (eTy ((tyApp (tyInd "List") (tyRel 0))))) (eLambda "x" (tyRel 1) (eApp (eApp (eConstr "List" "Cons_coq") (eTy (tyRel 0))) (eApp (eRel 1) (eRel 0))))) (eApp (eConstr "List" "Nil_coq") (eTy (tyRel 0)))))))
+ ;
+
+("foldl_alt", eTyLam "A" (eTyLam "A" (eLambda "x" (tyArr (tyRel 0) (tyArr (tyRel 1) (tyRel 0))) (eLetIn "f" (eFix "rec" "x" ((tyApp (tyInd "List") (tyRel 1))) (tyArr (tyRel 0) (tyRel 0)) (eLambda "x" (tyRel 0) (eCase ((tyApp (tyInd "List") (tyRel 1)), 0) (tyRel 0) (eRel 1) [(pConstr "Nil_coq" [], eRel 0);(pConstr "Cons_coq" ["x0";"x1"], eApp (eApp (eRel 4) (eRel 0)) (eApp (eApp (eRel 5) (eRel 2)) (eRel 1)))]))) (tyArr ((tyApp (tyInd "List") (tyRel 1))) (tyArr (tyRel 0) (tyRel 0))) (eRel 0)))))
+;("foldl", eTyLam "A" (eTyLam "A" (eLambda "x" (tyArr (tyRel 0) (tyArr (tyRel 1) (tyRel 0))) (eLambda "x" (tyRel 0) (eLambda "x" ((tyApp (tyInd "List") (tyRel 1))) (eApp (eApp (eApp (eApp (eApp (eConst "foldl_alt") (eTy (tyRel 1))) (eTy (tyRel 0))) (eRel 2)) (eRel 0)) (eRel 1)))))))
+ ;
+ ("concat", eTyLam "A" (eLambda "x" ((tyApp (tyInd "List") (tyRel 0))) (eLambda "x" ((tyApp (tyInd "List") (tyRel 0))) (eApp (eApp (eApp (eApp (eApp (eConst "foldr") (eTy (tyRel 0))) (eTy ((tyApp (tyInd "List") (tyRel 0))))) (eApp (eConstr "List" "Cons_coq") (eTy (tyRel 0)))) (eRel 0)) (eRel 1)))))
+;
+ ("zipWith", eTyLam "A" (eTyLam "A" (eTyLam "A" (eLambda "x" (tyArr (tyRel 2) (tyArr (tyRel 1) (tyRel 0))) (eLetIn "f" (eFix "rec" "x" ((tyApp (tyInd "List") (tyRel 2))) (tyArr ((tyApp (tyInd "List") (tyRel 1))) ((tyApp (tyInd "List") (tyRel 0)))) (eLambda "x" ((tyApp (tyInd "List") (tyRel 1))) (eCase ((tyApp (tyInd "List") (tyRel 2)), 0) ((tyApp (tyInd "List") (tyRel 0))) (eRel 1) [(pConstr "Nil_coq" [], eApp (eConstr "List" "Nil_coq") (eTy (tyRel 0)));(pConstr "Cons_coq" ["x0";"x1"], eCase ((tyApp (tyInd "List") (tyRel 1)), 0) ((tyApp (tyInd "List") (tyRel 0))) (eRel 2) [(pConstr "Nil_coq" [], eApp (eConstr "List" "Nil_coq") (eTy (tyRel 0)));(pConstr "Cons_coq" ["x0";"x1"], eApp (eApp (eApp (eConstr "List" "Cons_coq") (eTy (tyRel 0))) (eApp (eApp (eRel 7) (eRel 3)) (eRel 1))) (eApp (eApp (eRel 6) (eRel 2)) (eRel 0)))])]))) (tyArr ((tyApp (tyInd "List") (tyRel 2))) (tyArr ((tyApp (tyInd "List") (tyRel 1))) ((tyApp (tyInd "List") (tyRel 0))))) (eRel 0))))));
+("reverse", eTyLam "A" (eApp (eApp (eApp (eApp (eConst "foldl") (eTy (tyRel 0))) (eTy ((tyApp (tyInd "List") (tyRel 0))))) (eLambda "x" ((tyApp (tyInd "List") (tyRel 0))) (eLambda "x" (tyRel 0) (eApp (eApp (eApp (eConstr "List" "Cons_coq") (eTy (tyRel 0))) (eRel 0)) (eRel 1))))) (eApp (eConstr "List" "Nil_coq") (eTy (tyRel 0)))))
+;("zip", eTyLam "A" (eTyLam "A" (eApp (eApp (eApp (eApp (eConst "zipWith") (eTy (tyRel 1))) (eTy (tyRel 0))) (eTy ((tyApp (tyApp (tyInd "Pair") (tyRel 1)) (tyRel 0))))) (eApp (eApp (eConstr "Pair" "Pair_coq") (eTy (tyRel 1))) (eTy (tyRel 0))))))
+;("filter", eTyLam "A" (eLambda "x" (tyArr (tyRel 0) ((tyInd "Bool"))) (eApp (eApp (eApp (eApp (eConst "foldr") (eTy (tyRel 0))) (eTy ((tyApp (tyInd "List") (tyRel 0))))) (eLambda "x" (tyRel 0) (eLambda "x" ((tyApp (tyInd "List") (tyRel 0))) (eCase ((tyInd "Bool"), 0) ((tyApp (tyInd "List") (tyRel 0))) (eApp (eRel 2) (eRel 1)) [(pConstr "True_coq" [], eApp (eApp (eApp (eConstr "List" "Cons_coq") (eTy (tyRel 0))) (eRel 1)) (eRel 0));(pConstr "False_coq" [], eRel 0)])))) (eApp (eConstr "List" "Nil_coq") (eTy (tyRel 0))))))
+].
+
+  Run TemplateProgram (translateData ALB_data).
+
+  Definition gEnv := (StdLib.Σ ++ ALB_data ++ AcornMaybe.AM_data ++ AcornBool.AB_data ++ AcornProd.AP_data)%list.
+
+  Definition foldl_syn := eTyLam "A" (eTyLam "A" (eLambda "x" (tyArr (tyRel 0) (tyArr (tyRel 1) (tyRel 0))) (eLetIn "f" (eFix "rec" "x" (tyRel 0) (tyArr ((tyApp (tyInd "List") (tyRel 1))) (tyRel 0)) (eLambda "x" ((tyApp (tyInd "List") (tyRel 1))) (eCase ((tyApp (tyInd "List") (tyRel 1)), 0) (tyRel 0) (eRel 0) [(pConstr "Nil_coq" [], eRel 1);(pConstr "Cons_coq" ["x0";"x1"], eApp (eApp (eRel 4) (eApp (eApp (eRel 5) (eRel 3)) (eRel 1))) (eRel 0))]))) (tyArr (tyRel 0) (tyArr ((tyApp (tyInd "List") (tyRel 1))) (tyRel 0))) (eRel 0)))).
+
+  Compute (expr_to_term gEnv (reindexify 0 foldl_syn)).
+
+
+  Run TemplateProgram
+      (translateDefs gEnv ALB_functions).
+
+  Print foldr.
+  Print zipWith.
+End AcornListBase.
+
+Module AcornBlochain.
+
+  Definition ABl_data :=  [gdInd "Caller" 0 [("CallerContract_coq", [(TC.nAnon, tyInd "nat")]);("CallerAccount_coq", [(TC.nAnon, tyInd "string")])] false;gdInd "ChainContext" 0 [("ChainContext_coq", [(TC.nAnon, tyInd "nat");(TC.nAnon, tyInd "nat");(TC.nAnon, tyInd "nat")])] false;gdInd "InitContext" 0 [("InitContext_coq", [(TC.nAnon, (tyInd "ChainContext"));(TC.nAnon, tyInd "string")])] false;gdInd "ReceiveContext" 0 [("ReceiveContext_coq", [(TC.nAnon, (tyInd "ChainContext"));(TC.nAnon, tyInd "string");(TC.nAnon, tyInd "nat")])] false].
+
+  (*---------------------*)
+
+  Definition ABl_functions := [("slotNumber", eLambda "x" ((tyInd "ChainContext")) (eCase ((tyInd "ChainContext"), 0) (tyInd "nat") (eRel 0) [(pConstr "ChainContext_coq" ["x0";"x1";"x2"], eRel 2)]))
+;("blockHeight", eLambda "x" ((tyInd "ChainContext")) (eCase ((tyInd "ChainContext"), 0) (tyInd "nat") (eRel 0) [(pConstr "ChainContext_coq" ["x0";"x1";"x2"], eRel 1)]))
+;("finalizedHeight", eLambda "x" ((tyInd "ChainContext")) (eCase ((tyInd "ChainContext"), 0) (tyInd "nat") (eRel 0) [(pConstr "ChainContext_coq" ["x0";"x1";"x2"], eRel 0)]))
+;("initOrigin", eLambda "x" ((tyInd "InitContext")) (eCase ((tyInd "InitContext"), 0) (tyInd "string") (eRel 0) [(pConstr "InitContext_coq" ["x0";"x1"], eRel 0)]))
+;("initChain", eLambda "x" ((tyInd "InitContext")) (eCase ((tyInd "InitContext"), 0) ((tyInd "ChainContext")) (eRel 0) [(pConstr "InitContext_coq" ["x0";"x1"], eRel 1)]))
+;("receiveChain", eLambda "x" ((tyInd "ReceiveContext")) (eCase ((tyInd "ReceiveContext"), 0) ((tyInd "ChainContext")) (eRel 0) [(pConstr "ReceiveContext_coq" ["x0";"x1";"x2"], eRel 2)]))
+;("receiveOrigin", eLambda "x" ((tyInd "ReceiveContext")) (eCase ((tyInd "ReceiveContext"), 0) (tyInd "string") (eRel 0) [(pConstr "ReceiveContext_coq" ["x0";"x1";"x2"], eRel 1)]))
+;("receiveSelfAddress", eLambda "x" ((tyInd "ReceiveContext")) (eCase ((tyInd "ReceiveContext"), 0) (tyInd "nat") (eRel 0) [(pConstr "ReceiveContext_coq" ["x0";"x1";"x2"], eRel 0)]))].
+
+  Run TemplateProgram (translateData ABl_data).
+  Run TemplateProgram (translateDefs (StdLib.Σ ++ ABl_data)%list ABl_functions).
+End AcornBlochain.
 
 (** Concrete syntax *)
 
@@ -162,3 +239,69 @@ Definition count
               (owner x)
  end.
 End ForPeresentation.
+
+Module Recursion.
+
+  Definition R_data := [gdInd "Nat" 0 [("Zero_coq", []);("Suc_coq", [(TC.nAnon, (tyInd "Nat"))])] false].
+(*---------------------*)
+
+  Open Scope nat.
+
+  Definition R_functions := [("add", eLetIn "f" (eFix "rec" "x" ((tyInd "Nat")) (tyArr (tyInd "Nat") (tyInd "Nat")) (eLambda "x" ((tyInd "Nat")) (eCase ((tyInd "Nat"), 0) ((tyInd "Nat")) (eRel 1) [(pConstr "Zero_coq" [], eRel 0);(pConstr "Suc_coq" ["x0"], eApp (eConstr "Nat" "Suc_coq") (eApp (eApp (eRel 3) (eRel 0)) (eRel 1)))]))) (tyArr ((tyInd "Nat")) (tyArr (tyInd "Nat") (tyInd "Nat"))) (eRel 0))].
+
+  Run TemplateProgram (translateData R_data).
+
+  Run TemplateProgram (translateDefs (StdLib.Σ ++ R_data)%list R_functions).
+
+  Print add.
+
+
+
+  Fixpoint Nat_nat (n : Nat) : nat :=
+    match n with
+    | Zero_coq => O
+    | Suc_coq n' => S (Nat_nat n')
+    end.
+
+  Fixpoint nat_Nat (n : nat) : Nat :=
+    match n with
+    | O => Zero_coq
+    | S n' => Suc_coq (nat_Nat n')
+    end.
+
+  Lemma Nat_nat_left n : nat_Nat (Nat_nat n) = n.
+  Proof. induction n;simpl;f_equal;auto. Qed.
+
+
+  Lemma Nat_nat_right n : Nat_nat (nat_Nat n) = n.
+  Proof. induction n;simpl;f_equal;auto. Qed.
+
+  Hint Resolve Nat_nat_left Nat_nat_right : hints.
+
+  Local Coercion Nat_nat : Nat >-> nat.
+  Local Coercion nat_Nat : nat >-> Nat.
+
+  Lemma add_correct (n m : Nat) :
+  add n m = n + m.
+  Proof. induction n;simpl;f_equal;auto with hints. Qed.
+
+
+End Recursion.
+
+
+(** Predicativity *)
+Definition id := fun (A : Set) (a : A) => a.
+
+Definition id_id_syn := eApp (eApp (eConst "id") (eTy (tyForall "A" (tyArr (tyRel 0) (tyRel 0))))) (eConst "id").
+
+Compute (expr_to_term StdLib.Σ (reindexify 0 id_id_syn)).
+
+Eval compute in (expr_to_term StdLib.Σ (reindexify 0 id_id_syn)).
+
+Definition id_forall := eLambda "x" (tyForall "A" (tyArr (tyRel 0) (tyRel 0))) (eRel 0).
+
+Compute (expr_to_term StdLib.Σ (reindexify 0 id_forall)).
+
+(** Application [id id] fails, since [A] must be [Set], but type of
+ [id] is [forall A, A -> A], which lives in [Type]  *)
+Fail Make Definition id_id := Eval compute in (expr_to_term StdLib.Σ (reindexify 0 id_id_syn)).
